<?xml version="1.0"?>


<!DOCTYPE rdf:RDF [
    <!ENTITY owl "http://www.w3.org/2002/07/owl#" >
    <!ENTITY poddBase "http://purl.org/podd/ns/poddBase#" >
    <!ENTITY poddScience "http://purl.org/podd/ns/poddScience#" >
    <!ENTITY xsd "http://www.w3.org/2001/XMLSchema#" >
    <!ENTITY poddPlant "http://purl.org/podd/ns/poddPlant#" >
    <!ENTITY owl2xml "http://www.w3.org/2006/12/owl2-xml#" >
    <!ENTITY rdfs "http://www.w3.org/2000/01/rdf-schema#" >
    <!ENTITY rdf "http://www.w3.org/1999/02/22-rdf-syntax-ns#" >
]>


<rdf:RDF xmlns="http://purl.org/podd/ns/poddPlant#"
     xml:base="http://purl.org/podd/ns/poddPlant"
     xmlns:rdfs="http://www.w3.org/2000/01/rdf-schema#"
     xmlns:owl2xml="http://www.w3.org/2006/12/owl2-xml#"
     xmlns:poddPlant="http://purl.org/podd/ns/poddPlant#"
     xmlns:owl="http://www.w3.org/2002/07/owl#"
     xmlns:xsd="http://www.w3.org/2001/XMLSchema#"
     xmlns:rdf="http://www.w3.org/1999/02/22-rdf-syntax-ns#"
     xmlns:poddBase="http://purl.org/podd/ns/poddBase#"
     xmlns:poddScience="http://purl.org/podd/ns/poddScience#">
    <owl:Ontology rdf:about="http://purl.org/podd/ns/poddPlant">
        <owl:imports rdf:resource="http://purl.org/podd/ns/version/poddBase/1"/>
        <owl:imports rdf:resource="http://purl.org/podd/ns/version/poddScience/1"/>
        <owl:versionIRI rdf:resource="http://purl.org/podd/ns/version/poddPlant/1"/>
    </owl:Ontology>
    


    <!-- 
    ///////////////////////////////////////////////////////////////////////////////////////
    //
    // Annotation properties
    //
    ///////////////////////////////////////////////////////////////////////////////////////
     -->



    <!-- 
    ///////////////////////////////////////////////////////////////////////////////////////
    //
    // Object Properties
    //
    ///////////////////////////////////////////////////////////////////////////////////////
     -->

    


    <!-- http://purl.org/podd/ns/poddPlant#hasSubstrate -->

    <owl:ObjectProperty rdf:about="#hasSubstrate">
        <rdfs:label>Substrate</rdfs:label>
        <rdfs:range rdf:resource="#Substrate"/>
        <poddBase:weight>7</poddBase:weight>
    </owl:ObjectProperty>
    


    <!-- 
    ///////////////////////////////////////////////////////////////////////////////////////
    //
    // Data properties
    //
    ///////////////////////////////////////////////////////////////////////////////////////
     -->

    


    <!-- http://purl.org/podd/ns/poddScience#hasName -->

    <owl:DatatypeProperty rdf:about="&poddScience;hasName"/>
    


    <!-- http://purl.org/podd/ns/poddPlant#hasEcotype -->

    <owl:DatatypeProperty rdf:about="#hasEcotype">
        <rdfs:label>Ecotype</rdfs:label>
        <rdfs:range rdf:resource="&xsd;string"/>
        <poddBase:weight>10</poddBase:weight>
    </owl:DatatypeProperty>
    


    <!-- http://purl.org/podd/ns/poddPlant#hasFieldDescription -->

    <owl:DatatypeProperty rdf:about="#hasFieldDescription">
        <rdfs:label
            >Field Description</rdfs:label>
        <rdfs:range rdf:resource="&xsd;string"/>
        <poddBase:weight>10</poddBase:weight>
    </owl:DatatypeProperty>
    


    <!-- http://purl.org/podd/ns/poddPlant#hasFieldSoilType -->

    <owl:DatatypeProperty rdf:about="#hasFieldSoilType">
        <rdfs:label>Field Soil Type</rdfs:label>
        <rdfs:range rdf:resource="&xsd;string"/>
        <poddBase:weight>7</poddBase:weight>
    </owl:DatatypeProperty>
    


    <!-- 
    ///////////////////////////////////////////////////////////////////////////////////////
    //
    // Classes
    //
    ///////////////////////////////////////////////////////////////////////////////////////
     -->

    


    <!-- http://purl.org/podd/ns/poddScience#ANZSRC -->

    <owl:Class rdf:about="&poddScience;ANZSRC">
        <owl:equivalentClass>
            <owl:Class>
                <owl:oneOf rdf:parseType="Collection">
                    <rdf:Description rdf:about="#ANZSRC07-Agriculture-and-Veterinary-Sciences"/>
                    <rdf:Description rdf:about="#ANZSRC-NotApplicable"/>
                    <rdf:Description rdf:about="#ANZSRC06-Biological-Sciences"/>
                </owl:oneOf>
            </owl:Class>
        </owl:equivalentClass>
    </owl:Class>
    


    <!-- http://purl.org/podd/ns/poddScience#Environment -->

    <owl:Class rdf:about="&poddScience;Environment"/>
    


    <!-- http://purl.org/podd/ns/poddScience#Genotype -->

    <owl:Class rdf:about="&poddScience;Genotype">
        <rdfs:subClassOf>
            <owl:Restriction>
                <owl:onProperty rdf:resource="#hasEcotype"/>
                <owl:allValuesFrom rdf:resource="&xsd;string"/>
            </owl:Restriction>
        </rdfs:subClassOf>
    </owl:Class>
    


    <!-- http://purl.org/podd/ns/poddPlant#FieldConditions -->

    <owl:Class rdf:about="#FieldConditions">
        <rdfs:label
            >Field Conditions</rdfs:label>
        <rdfs:subClassOf rdf:resource="&poddScience;Environment"/>
        <rdfs:subClassOf>
            <owl:Restriction>
                <owl:onProperty rdf:resource="#hasFieldDescription"/>
                <owl:allValuesFrom rdf:resource="&xsd;string"/>
            </owl:Restriction>
        </rdfs:subClassOf>
        <rdfs:subClassOf>
            <owl:Restriction>
                <owl:onProperty rdf:resource="#hasFieldSoilType"/>
                <owl:allValuesFrom rdf:resource="&xsd;string"/>
            </owl:Restriction>
        </rdfs:subClassOf>
    </owl:Class>
    


    <!-- http://purl.org/podd/ns/poddPlant#GrowthConditions -->

    <owl:Class rdf:about="#GrowthConditions">
        <rdfs:label
            >Growth Conditions</rdfs:label>
        <rdfs:subClassOf rdf:resource="&poddScience;Environment"/>
        <rdfs:subClassOf>
            <owl:Restriction>
                <owl:onProperty rdf:resource="#hasSubstrate"/>
                <owl:allValuesFrom rdf:resource="#Substrate"/>
            </owl:Restriction>
        </rdfs:subClassOf>
    </owl:Class>
    


    <!-- http://purl.org/podd/ns/poddPlant#Substrate -->

    <owl:Class rdf:about="#Substrate">
        <rdfs:label>Substrate</rdfs:label>
        <rdfs:subClassOf>
            <owl:Restriction>
                <owl:onProperty rdf:resource="&poddScience;hasName"/>
                <owl:qualifiedCardinality rdf:datatype="&xsd;nonNegativeInteger">1</owl:qualifiedCardinality>
                <owl:onDataRange rdf:resource="&xsd;string"/>
            </owl:Restriction>
        </rdfs:subClassOf>
        <rdfs:subClassOf>
            <owl:Restriction>
                <owl:onProperty rdf:resource="&poddBase;hasDescription"/>
                <owl:maxQualifiedCardinality rdf:datatype="&xsd;nonNegativeInteger">1</owl:maxQualifiedCardinality>
                <owl:onDataRange rdf:resource="&xsd;string"/>
            </owl:Restriction>
        </rdfs:subClassOf>
    </owl:Class>
    


    <!-- http://www.w3.org/2002/07/owl#Thing -->

    <owl:Class rdf:about="&owl;Thing"/>
    


    <!-- 
    ///////////////////////////////////////////////////////////////////////////////////////
    //
    // Individuals
    //
    ///////////////////////////////////////////////////////////////////////////////////////
     -->

    


    <!-- http://purl.org/podd/ns/poddPlant#ANZSRC-NotApplicable -->

    <owl:Thing rdf:about="#ANZSRC-NotApplicable">
        <rdf:type rdf:resource="&poddScience;ANZSRC"/>
        <poddBase:weight>1</poddBase:weight>
    </owl:Thing>
    


    <!-- http://purl.org/podd/ns/poddPlant#ANZSRC06-Biological-Sciences -->

    <owl:Thing rdf:about="#ANZSRC06-Biological-Sciences">
        <rdf:type rdf:resource="&poddScience;ANZSRC"/>
        <poddBase:weight>2</poddBase:weight>
    </owl:Thing>
    


    <!-- http://purl.org/podd/ns/poddPlant#ANZSRC07-Agriculture-and-Veterinary-Sciences -->

    <owl:Thing rdf:about="#ANZSRC07-Agriculture-and-Veterinary-Sciences">
        <rdf:type rdf:resource="&poddScience;ANZSRC"/>
        <poddBase:weight>3</poddBase:weight>
    </owl:Thing>

<rdf:Description rdf:about="http://purl.org/podd/ns/poddPlant#Closedfluorescencesystem-e1cd2381-64c6-4dc3-b3c3-e0aae07a5d8d">
	<rdf:type rdf:resource="http://www.w3.org/2002/07/owl#Thing"/>
	<rdf:type rdf:resource="http://www.w3.org/2002/07/owl#NamedIndividual"/>
	<rdf:type rdf:resource="http://purl.org/podd/ns/poddScience#Platform"/>
	<poddScience:hasPlatformType rdf:resource="http://purl.org/podd/ns/poddScience#Hardware"/>
	<rdfs:label>Closed fluorescence system</rdfs:label>
	<rdfs:comment>Closed imaging fluorescence system</rdfs:comment>
</rdf:Description>

<rdf:Description rdf:about="http://purl.org/podd/ns/poddPlant#DeltaTporometer-a95133f9-58cc-418e-abc2-82e6233be04c">
	<rdf:type rdf:resource="http://www.w3.org/2002/07/owl#Thing"/>
	<rdf:type rdf:resource="http://www.w3.org/2002/07/owl#NamedIndividual"/>
	<rdf:type rdf:resource="http://purl.org/podd/ns/poddScience#Platform"/>
	<poddScience:hasPlatformType rdf:resource="http://purl.org/podd/ns/poddScience#Hardware"/>
	<rdfs:label>Delta-T porometer</rdfs:label>
	<rdfs:comment>This hand held device performs non-destructive measurements of stomatal conductance in plant leaf tissue.</rdfs:comment>
</rdf:Description>

<rdf:Description rdf:about="http://purl.org/podd/ns/poddPlant#FieldScoutCM1000-10d13dad-4f38-4e17-b33b-328d670f314f">
	<rdf:type rdf:resource="http://www.w3.org/2002/07/owl#Thing"/>
	<rdf:type rdf:resource="http://www.w3.org/2002/07/owl#NamedIndividual"/>
	<rdf:type rdf:resource="http://purl.org/podd/ns/poddScience#Platform"/>
	<poddScience:hasPlatformType rdf:resource="http://purl.org/podd/ns/poddScience#Hardware"/>
	<rdfs:label>Field Scout CM-1000</rdfs:label>
	<rdfs:comment>This hand held device performs non-destructive measurements of the chlorophyll content of leaves and canopies using reflectance.</rdfs:comment>
</rdf:Description>

<rdf:Description rdf:about="http://purl.org/podd/ns/poddPlant#FLIRI7InfraredthermographyCamera-22bf7c49-4e2b-47b7-beae-290b8657417f">
	<rdf:type rdf:resource="http://www.w3.org/2002/07/owl#Thing"/>
	<rdf:type rdf:resource="http://www.w3.org/2002/07/owl#NamedIndividual"/>
	<rdf:type rdf:resource="http://purl.org/podd/ns/poddScience#Platform"/>
	<poddScience:hasPlatformType rdf:resource="http://purl.org/podd/ns/poddScience#Hardware"/>
	<rdfs:label>FLIR I7 - Infrared thermography Camera</rdfs:label>
	<rdfs:comment>This is a hand held infrared video camera. Used for assessing temperature at the leaf, plant or field level.</rdfs:comment>
</rdf:Description>

<rdf:Description rdf:about="http://purl.org/podd/ns/poddPlant#FLIRSC660InfraredThermographyCameraandDellPrecisionLaptop-fa5bf077-bcc1-4510-b20c-ad7e5e46945f">
	<rdf:type rdf:resource="http://www.w3.org/2002/07/owl#Thing"/>
	<rdf:type rdf:resource="http://www.w3.org/2002/07/owl#NamedIndividual"/>
	<rdf:type rdf:resource="http://purl.org/podd/ns/poddScience#Platform"/>
	<poddScience:hasPlatformType rdf:resource="http://purl.org/podd/ns/poddScience#Hardware"/>
	<rdfs:label>FLIR-SC660 Infrared Thermography Camera and Dell Precision Laptop</rdfs:label>
	<rdfs:comment>This is a hand held infrared video camera. Used for assessing temperature at the leaf, plant or field level. It comes with a DELL precision computer with ThermaCAM Researcher</rdfs:comment>
</rdf:Description>

<rdf:Description rdf:about="http://purl.org/podd/ns/poddPlant#FTIRMicroscope-d32c879e-58d3-4069-82db-2fbfb7987615">
	<rdf:type rdf:resource="http://www.w3.org/2002/07/owl#Thing"/>
	<rdf:type rdf:resource="http://www.w3.org/2002/07/owl#NamedIndividual"/>
	<rdf:type rdf:resource="http://purl.org/podd/ns/poddScience#Platform"/>
	<poddScience:hasPlatformType rdf:resource="http://purl.org/podd/ns/poddScience#Hardware"/>
	<rdfs:label>FTIR Microscope</rdfs:label>
	<rdfs:comment>Fourier Transformation InfraRed microscope. It performs analysis of chemical composition of plant cells and associates these with images.</rdfs:comment>
</rdf:Description>

<rdf:Description rdf:about="http://purl.org/podd/ns/poddPlant#HyperspectralReflectanceRadiometerCalibratedlabsystem-beb4d8e7-b1c9-4a8d-95f5-40f4170455ae">
	<rdf:type rdf:resource="http://www.w3.org/2002/07/owl#Thing"/>
	<rdf:type rdf:resource="http://www.w3.org/2002/07/owl#NamedIndividual"/>
	<rdf:type rdf:resource="http://purl.org/podd/ns/poddScience#Platform"/>
	<poddScience:hasPlatformType rdf:resource="http://purl.org/podd/ns/poddScience#Hardware"/>
	<rdfs:label>Hyperspectral Reflectance Radiometer</rdfs:label>
	<rdfs:comment>This platform collects spectra information, and consequently supports the analysis of chemical composition.</rdfs:comment>
</rdf:Description>

<rdf:Description rdf:about="http://purl.org/podd/ns/poddPlant#IntegratingSphereASDforeoptics-a95e1536-3fa0-410d-9f02-a5fd0b5625eb">
	<rdf:type rdf:resource="http://www.w3.org/2002/07/owl#Thing"/>
	<rdf:type rdf:resource="http://www.w3.org/2002/07/owl#NamedIndividual"/>
	<rdf:type rdf:resource="http://purl.org/podd/ns/poddScience#Platform"/>
	<poddScience:hasPlatformType rdf:resource="http://purl.org/podd/ns/poddScience#Hardware"/>
	<rdfs:label>Integrating Sphere (ASD foreoptics)</rdfs:label>
	<rdfs:comment>Integrating sphere for ASD hyperspectral radiometer</rdfs:comment>
</rdf:Description>

<rdf:Description rdf:about="http://purl.org/podd/ns/poddPlant#LeafAreaMeter-bd7dc432-7943-4f95-807c-8e74aa98253b">
	<rdf:type rdf:resource="http://www.w3.org/2002/07/owl#Thing"/>
	<rdf:type rdf:resource="http://www.w3.org/2002/07/owl#NamedIndividual"/>
	<rdf:type rdf:resource="http://purl.org/podd/ns/poddScience#Platform"/>
	<poddScience:hasPlatformType rdf:resource="http://purl.org/podd/ns/poddScience#Hardware"/>
	<rdfs:label>Leaf Area Meter</rdfs:label>
	<rdfs:comment>Gives data output of leaf area, can be used as a portable system or in combination with a conveyor system for higher throughput analysis</rdfs:comment>
</rdf:Description>

<rdf:Description rdf:about="http://purl.org/podd/ns/poddPlant#LemnaTecScanalyserUpstairs-445c16bc-83e1-4c69-95c3-ca8670700166">
	<rdf:type rdf:resource="http://www.w3.org/2002/07/owl#Thing"/>
	<rdf:type rdf:resource="http://www.w3.org/2002/07/owl#NamedIndividual"/>
	<rdf:type rdf:resource="http://purl.org/podd/ns/poddScience#Platform"/>
	<poddScience:hasPlatformType rdf:resource="http://purl.org/podd/ns/poddScience#Hardware"/>
	<rdfs:label>LemnaTec Scanalyser</rdfs:label>
	<rdfs:comment>The Lemnatec Scanalyser is an optical imaging system that uses a camera to take visible spectrum images of a plant and then provide analysis of individual plants or series of images.</rdfs:comment>
</rdf:Description>

<rdf:Description rdf:about="http://purl.org/podd/ns/poddPlant#LemnatecscanalyserNIR-c5cfcfdc-acb9-4983-a110-5663590909d0">
	<rdf:type rdf:resource="http://www.w3.org/2002/07/owl#Thing"/>
	<rdf:type rdf:resource="http://www.w3.org/2002/07/owl#NamedIndividual"/>
	<rdf:type rdf:resource="http://purl.org/podd/ns/poddScience#Platform"/>
	<poddScience:hasPlatformType rdf:resource="http://purl.org/podd/ns/poddScience#Hardware"/>
	<rdfs:label>Lemnatec scanalyser (NIR)</rdfs:label>
	<rdfs:comment>The Lemnatec Scanalyser is an optical imaging system that uses a camera to take visible and NIR spectrum images of a plant and then provide analysis of individual plants or series of images.</rdfs:comment>
</rdf:Description>

<rdf:Description rdf:about="http://purl.org/podd/ns/poddPlant#LICOR64001-f72e8863-dc2b-4209-adb8-62df9c4f626e">
	<rdf:type rdf:resource="http://www.w3.org/2002/07/owl#Thing"/>
	<rdf:type rdf:resource="http://www.w3.org/2002/07/owl#NamedIndividual"/>
	<rdf:type rdf:resource="http://purl.org/podd/ns/poddScience#Platform"/>
	<poddScience:hasPlatformType rdf:resource="http://purl.org/podd/ns/poddScience#Hardware"/>
	<rdfs:label>LI-COR 6400</rdfs:label>
	<rdfs:comment>This is a non imaging device that performs gas exchange analysis used to make photosynthesis measurements. It is portable and can be used for indoor or outdoor measurements.</rdfs:comment>
</rdf:Description>

<rdf:Description rdf:about="http://purl.org/podd/ns/poddPlant#Linequantumsensor1-022b6a39-db44-4c6d-8607-af45d05b1763">
	<rdf:type rdf:resource="http://www.w3.org/2002/07/owl#Thing"/>
	<rdf:type rdf:resource="http://www.w3.org/2002/07/owl#NamedIndividual"/>
	<rdf:type rdf:resource="http://purl.org/podd/ns/poddScience#Platform"/>
	<poddScience:hasPlatformType rdf:resource="http://purl.org/podd/ns/poddScience#Hardware"/>
	<rdfs:label>Line quantum sensor</rdfs:label>
	<rdfs:comment>This hand-held system performs non-destructive PAR light interception measurements.</rdfs:comment>
</rdf:Description>

<rdf:Description rdf:about="http://purl.org/podd/ns/poddPlant#MonitoringPAM-10171360-8e9b-4dbc-bd3a-17cbc88dac7a">
	<rdf:type rdf:resource="http://www.w3.org/2002/07/owl#Thing"/>
	<rdf:type rdf:resource="http://www.w3.org/2002/07/owl#NamedIndividual"/>
	<rdf:type rdf:resource="http://purl.org/podd/ns/poddScience#Platform"/>
	<poddScience:hasPlatformType rdf:resource="http://purl.org/podd/ns/poddScience#Hardware"/>
	<rdfs:label>Monitoring PAM</rdfs:label>
	<rdfs:comment>This equipment is restricted to trained users - please contact a staff member to organise training</rdfs:comment>
</rdf:Description>

<rdf:Description rdf:about="http://purl.org/podd/ns/poddPlant#Openfluorescencesystem-9c87f1bf-b29d-4f61-8063-3490ef14b767">
	<rdf:type rdf:resource="http://www.w3.org/2002/07/owl#Thing"/>
	<rdf:type rdf:resource="http://www.w3.org/2002/07/owl#NamedIndividual"/>
	<rdf:type rdf:resource="http://purl.org/podd/ns/poddScience#Platform"/>
	<poddScience:hasPlatformType rdf:resource="http://purl.org/podd/ns/poddScience#Hardware"/>
	<rdfs:label>Open fluorescence system</rdfs:label>
	<rdfs:comment>Imaging fluorescence system</rdfs:comment>
</rdf:Description>

<rdf:Description rdf:about="http://purl.org/podd/ns/poddPlant#PAM2500-84d5dd24-de9a-4525-bdc9-e7a53ce239d8">
	<rdf:type rdf:resource="http://www.w3.org/2002/07/owl#Thing"/>
	<rdf:type rdf:resource="http://www.w3.org/2002/07/owl#NamedIndividual"/>
	<rdf:type rdf:resource="http://purl.org/podd/ns/poddScience#Platform"/>
	<poddScience:hasPlatformType rdf:resource="http://purl.org/podd/ns/poddScience#Hardware"/>
	<rdfs:label>PAM 2500</rdfs:label>
	<rdfs:comment>Non-imaging fluorescence system</rdfs:comment>
</rdf:Description>

<rdf:Description rdf:about="http://purl.org/podd/ns/poddPlant#PSIFP100-a535014c-89f4-47a4-8656-5252ff75f75d">
	<rdf:type rdf:resource="http://www.w3.org/2002/07/owl#Thing"/>
	<rdf:type rdf:resource="http://www.w3.org/2002/07/owl#NamedIndividual"/>
	<rdf:type rdf:resource="http://purl.org/podd/ns/poddScience#Platform"/>
	<poddScience:hasPlatformType rdf:resource="http://purl.org/podd/ns/poddScience#Hardware"/>
	<rdfs:label>PSI FP100</rdfs:label>
	<rdfs:comment>This hand-held system performs non-destructive fluorescence measurements.</rdfs:comment>
</rdf:Description>

<rdf:Description rdf:about="http://purl.org/podd/ns/poddPlant#PSINDVI1-3a3c63e0-ca0e-4d46-ab6b-732c4a5e3e76">
	<rdf:type rdf:resource="http://www.w3.org/2002/07/owl#Thing"/>
	<rdf:type rdf:resource="http://www.w3.org/2002/07/owl#NamedIndividual"/>
	<rdf:type rdf:resource="http://purl.org/podd/ns/poddScience#Platform"/>
	<poddScience:hasPlatformType rdf:resource="http://purl.org/podd/ns/poddScience#Hardware"/>
	<rdfs:label>PSI NDVI</rdfs:label>
	<rdfs:comment>This hand-held system performs non-destructive NDVI measurements.</rdfs:comment>
</rdf:Description>

<rdf:Description rdf:about="http://purl.org/podd/ns/poddPlant#PSIPRI1-283744de-d21a-47c7-a98f-485d057318ed">
	<rdf:type rdf:resource="http://www.w3.org/2002/07/owl#Thing"/>
	<rdf:type rdf:resource="http://www.w3.org/2002/07/owl#NamedIndividual"/>
	<rdf:type rdf:resource="http://purl.org/podd/ns/poddScience#Platform"/>
	<poddScience:hasPlatformType rdf:resource="http://purl.org/podd/ns/poddScience#Hardware"/>
	<rdfs:label>PSI PRI</rdfs:label>
	<rdfs:comment>This hand-held system performs non-destructive PRI measurements.</rdfs:comment>
</rdf:Description>

<rdf:Description rdf:about="http://purl.org/podd/ns/poddPlant#Pyrometer1-9ea9f3ae-a290-4bb2-98b0-a67c766da520">
	<rdf:type rdf:resource="http://www.w3.org/2002/07/owl#Thing"/>
	<rdf:type rdf:resource="http://www.w3.org/2002/07/owl#NamedIndividual"/>
	<rdf:type rdf:resource="http://purl.org/podd/ns/poddScience#Platform"/>
	<poddScience:hasPlatformType rdf:resource="http://purl.org/podd/ns/poddScience#Hardware"/>
	<rdfs:label>Pyrometer</rdfs:label>
	<rdfs:comment>This hand held device performs non-contact temperature measurements</rdfs:comment>
</rdf:Description>

<rdf:Description rdf:about="http://purl.org/podd/ns/poddPlant#PyrometerAgriThermIII-4cd1c85c-b95d-4705-89c7-533cf1f2b07a">
	<rdf:type rdf:resource="http://www.w3.org/2002/07/owl#Thing"/>
	<rdf:type rdf:resource="http://www.w3.org/2002/07/owl#NamedIndividual"/>
	<rdf:type rdf:resource="http://purl.org/podd/ns/poddScience#Platform"/>
	<poddScience:hasPlatformType rdf:resource="http://purl.org/podd/ns/poddScience#Hardware"/>
	<rdfs:label>Pyrometer (AgriTherm III)</rdfs:label>
	<rdfs:comment>This hand held device performs non-contact temperature measurements</rdfs:comment>
</rdf:Description>

<rdf:Description rdf:about="http://purl.org/podd/ns/poddPlant#SC1Porometer-31e2a189-dcab-4df5-869e-b38a1c3e938a">
	<rdf:type rdf:resource="http://www.w3.org/2002/07/owl#Thing"/>
	<rdf:type rdf:resource="http://www.w3.org/2002/07/owl#NamedIndividual"/>
	<rdf:type rdf:resource="http://purl.org/podd/ns/poddScience#Platform"/>
	<poddScience:hasPlatformType rdf:resource="http://purl.org/podd/ns/poddScience#Hardware"/>
	<rdfs:label>SC1 Porometer</rdfs:label>
	<rdfs:comment>This hand held device performs non-destructive measurements of stomatal conductance in plant leaf tissue.</rdfs:comment>
</rdf:Description>

<rdf:Description rdf:about="http://purl.org/podd/ns/poddPlant#ShootRootApparatus-3807f063-8a0a-4c5e-a2a1-e1cc1fc9872c">
	<rdf:type rdf:resource="http://www.w3.org/2002/07/owl#Thing"/>
	<rdf:type rdf:resource="http://www.w3.org/2002/07/owl#NamedIndividual"/>
	<rdf:type rdf:resource="http://purl.org/podd/ns/poddScience#Platform"/>
	<poddScience:hasPlatformType rdf:resource="http://purl.org/podd/ns/poddScience#Hardware"/>
	<rdfs:label>Shoot Root Apparatus</rdfs:label>
	<rdfs:comment>This system records plant growth in controlled environments (i.e. growth cabinets), through the use of 3 Point Grey digital cameras.</rdfs:comment>
</rdf:Description>

<rdf:Description rdf:about="http://purl.org/podd/ns/poddPlant#SPADMeter-7c00463a-b46b-4cb1-b0d3-f756d9956875">
	<rdf:type rdf:resource="http://www.w3.org/2002/07/owl#Thing"/>
	<rdf:type rdf:resource="http://www.w3.org/2002/07/owl#NamedIndividual"/>
	<rdf:type rdf:resource="http://purl.org/podd/ns/poddScience#Platform"/>
	<poddScience:hasPlatformType rdf:resource="http://purl.org/podd/ns/poddScience#Hardware"/>
	<rdfs:label>SPAD Meter</rdfs:label>
	<rdfs:comment>This hand held device performs non-destructive measurements of the chlorophyll content of plant leaves using absorption.</rdfs:comment>
</rdf:Description>

<rdf:Description rdf:about="http://purl.org/podd/ns/poddPlant#Trayscan-f1e00952-fde7-4a8d-a79a-34eeb8ed2213">
	<rdf:type rdf:resource="http://www.w3.org/2002/07/owl#Thing"/>
	<rdf:type rdf:resource="http://www.w3.org/2002/07/owl#NamedIndividual"/>
	<rdf:type rdf:resource="http://purl.org/podd/ns/poddScience#Platform"/>
	<poddScience:hasPlatformType rdf:resource="http://purl.org/podd/ns/poddScience#Hardware"/>
	<rdfs:label>Trayscan</rdfs:label>
	<rdfs:comment>System to measure IR, Fluorescence and RGB simultaneously - medium to high throughput</rdfs:comment>
</rdf:Description>
</rdf:RDF>



<!-- Generated by the OWL API (version 2.2.1.1138) http://owlapi.sourceforge.net -->

